Pcc116Code/Imp.lean
@@ -1,0 +1,289 @@
+import Mathlib.Data.Nat.Defs 
+import Mathlib.Tactic.Basic 
+import Aesop
+import Lean.Elab.Tactic
+
+open Lean Elab Meta
+
+-- literals 
+
+inductive Lit : Type
+| INat : ℕ → Lit 
+
+-- operators 
+
+inductive Unop : Type 
+| Unot : Unop
+
+inductive Binop : Type 
+| BPlus : Binop 
+| BAnd  : Binop 
+| BLess : Binop 
+
+-- expressions 
+
+inductive IExp : Type 
+| ELit : Lit → IExp 
+| EVar : String → IExp 
+| EUn : Unop → IExp → IExp 
+| BOp : Binop → IExp → IExp → IExp 
+
+-- programs 
+
+inductive Stmt : Type 
+| Skip : Stmt 
+| Assign : String → IExp → Stmt 
+| Seq : Stmt → Stmt → Stmt 
+| If : IExp → Stmt → Stmt → Stmt 
+| While : IExp → Stmt → Stmt 
+
+-- elaborating syntax using macros 
+
+declare_syntax_cat imp_lit
+
+syntax num : imp_lit
+syntax "true" : imp_lit
+syntax "false" : imp_lit
+
+def elabLit : Syntax → MetaM Expr 
+| `(imp_lit| $n:num) => mkAppM ``Lit.INat #[mkNatLit n.getNat]
+| `(imp_lit| true) => mkAppM ``Lit.INat #[mkNatLit 1]
+| `(imp_lit| false) => mkAppM ``Lit.INat #[mkNatLit 0]
+| _ => throwUnsupportedSyntax
+
+elab "test_elabLit" l:imp_lit : term => elabLit l
+
+#reduce test_elabLit 3 
+#reduce test_elabLit true 
+
+declare_syntax_cat imp_unop
+
+syntax "not" : imp_unop 
+
+def elabUnop : Syntax → MetaM Expr 
+| `(imp_unop| not) => return .const ``Unop.Unot []
+| _ => throwUnsupportedSyntax
+
+declare_syntax_cat imp_bin_op 
+
+syntax "+" : imp_bin_op
+syntax "and" : imp_bin_op
+syntax "<" : imp_bin_op
+
+def elabBinop : Syntax → MetaM Expr 
+| `(imp_bin_op| +) => return .const ``Binop.BPlus []
+| `(imp_bin_op| and) => return .const ``Binop.BAnd []
+| `(imp_bin_op| <) => return .const ``Binop.BLess []
+| _ => throwUnsupportedSyntax
+
+-- elaborating expressions 
+
+declare_syntax_cat imp_exp 
+
+syntax imp_lit : imp_exp 
+syntax ident : imp_exp 
+syntax imp_unop imp_exp : imp_exp 
+syntax imp_exp imp_bin_op imp_exp : imp_exp 
+
+syntax "(" imp_exp ")" : imp_exp 
+
+partial def elabExp : Syntax → MetaM Expr 
+| `(imp_exp| $l:imp_lit) => do 
+  let l ← elabLit l 
+  mkAppM ``IExp.ELit #[l] 
+| `(imp_exp| $i:ident) => 
+  mkAppM ``IExp.EVar #[mkStrLit i.getId.toString]
+| `(imp_exp| $b:imp_unop $e:imp_exp) => do 
+  let b ← elabUnop b 
+  let e ← elabExp e 
+  mkAppM ``IExp.EUn #[b,e]
+| `(imp_exp| $l:imp_exp $b:imp_bin_op $r:imp_exp) => do 
+  let l ← elabExp l 
+  let b ← elabBinop b 
+  let r ← elabExp r 
+  mkAppM ``IExp.BOp #[b, l, r]
+| `(imp_exp| ($e:imp_exp)) => 
+  elabExp e
+| _ => throwUnsupportedSyntax 
+
+elab "test_elabExp" e:imp_exp : term => elabExp e 
+
+#reduce test_elabExp a + 3
+
+-- statements 
+
+declare_syntax_cat imp_stmt 
+
+syntax "skip" : imp_stmt 
+syntax ident ":=" imp_exp : imp_stmt 
+syntax imp_stmt ";;" imp_stmt : imp_stmt 
+syntax "if" imp_exp "then" imp_stmt "else" imp_stmt "fi" : imp_stmt 
+syntax "while" imp_exp "do" imp_stmt "od" : imp_stmt 
+
+partial def elabStmt : Syntax → MetaM Expr 
+| `(imp_stmt| skip) => return .const ``Stmt.Skip []
+| `(imp_stmt| $i:ident := $e:imp_exp) => do 
+  let i : Expr := mkStrLit i.getId.toString
+  let e ← elabExp e 
+  mkAppM ``Stmt.Assign #[i, e]
+| `(imp_stmt| $s1:imp_stmt ;; $s2:imp_stmt) => do 
+  let s1 ← elabStmt s1 
+  let s2 ← elabStmt s2 
+  mkAppM ``Stmt.Seq #[s1, s2]
+| `(imp_stmt| if $e:imp_exp then $s1:imp_stmt else $s2:imp_stmt fi) => do 
+  let e ← elabExp e 
+  let s1 ← elabStmt s1 
+  let s2 ← elabStmt s2 
+  mkAppM ``Stmt.If #[e,s1,s2]
+| `(imp_stmt| while $e:imp_exp do $s:imp_stmt od) => do 
+  let e ← elabExp e 
+  let s ← elabStmt s 
+  mkAppM ``Stmt.While #[e, s]
+| _ => throwUnsupportedSyntax
+
+elab "{imp|" p: imp_stmt "}" : term => elabStmt p
+
+#reduce {imp|
+  a := 5 ;; 
+  if a < 3 and a < 1 then 
+    c := 5
+  else 
+    skip 
+  fi ;;  
+  d := c + 3  
+}
+
+-- environments 
+
+abbrev Value := ℕ 
+
+inductive Result (A : Type) : Type where 
+| Ok : A → Result A 
+| TypeError : Result A 
+| OutOfFuel : Result A  
+
+-- semantics of expressions 
+
+abbrev Env := String → Value 
+
+def emptyEnv : Env := λ _ => 0
+
+def updateEnv : String → Value → Env → Env
+| s, v, env => λ s' =>
+  if Substring.beq s.toSubstring s'.toSubstring
+  then v
+  else env s
+
+macro  x:term "|->" v:term ";" s:term  : term => 
+  `(updateEnv $x $v $s)
+
+def vlt (n1 n2 : Value) : Value := 
+  if Nat.blt n1 n2 then 1 else 0
+
+def vand (n1 n2 : Value) : Value := 
+  if Nat.beq n1 0 then 0 else n2 
+
+def vnot (n1 : Value) : Value := 
+  if Nat.ble n1 0 then 1 else 0  
+
+def evalBOp : Binop → Value → Value → Value
+| Binop.BPlus => λ x y => x + y  
+| Binop.BLess => vlt 
+| Binop.BAnd => vand  
+
+def evalExp : IExp → Env → Value
+| IExp.ELit (Lit.INat l), _ => l 
+| IExp.EVar v, env => env v
+| IExp.EUn _ e1, env => vnot (evalExp e1 env)
+| IExp.BOp op e1 e2, env => 
+  (evalBOp op) (evalExp e1 env) (evalExp e2 env)
+
+abbrev Fuel := ℕ
+
+def evalStmt : Fuel → Stmt → Env → Result Env 
+| 0 , _ , _ => Result.OutOfFuel
+| _ + 1, Stmt.Skip , env => Result.Ok env 
+| _ + 1, Stmt.Assign v e, env =>
+  Result.Ok (v |-> (evalExp e env) ; env)
+| fuel' + 1, Stmt.Seq s1 s2, env => 
+  match evalStmt fuel' s1 env with 
+  | Result.Ok env1 => evalStmt fuel' s2 env1
+  | r => r 
+| fuel' + 1, Stmt.If e s1 s2, env => 
+  match evalExp e env with 
+  | 0 => 
+    evalStmt fuel' s2 env 
+  | _ + 1 => 
+    evalStmt fuel' s1 env 
+| fuel' + 1, Stmt.While e s1, env => 
+  match evalExp e env with 
+  | _ + 1 => 
+    match evalStmt fuel' s1 env with 
+    | Result.Ok env1 => 
+      evalStmt fuel' (Stmt.While e s1) env1
+    | r => r 
+  | 0 => Result.Ok env 
+
+-- semantics of statements 
+
+inductive Eval : Env → Stmt → Env → Prop
+| ESkip : ∀ env, Eval env Stmt.Skip env
+| EAssign : ∀ env s e v,
+            evalExp e env = v →
+            Eval env (Stmt.Assign s e) (s |-> v ; env)
+| ESeq : ∀ env env1 env2 s1 s2,
+           Eval env s1 env1 →
+           Eval env1 s2 env2 →
+           Eval env (Stmt.Seq s1 s2) env2
+| EIfTrue : ∀ env e s1 s2 env1 n,
+            evalExp e env = n + 1 →
+            Eval env s1 env1 →
+            Eval env (Stmt.If e s1 s2) env1
+| EIfFalse : ∀ env e s1 s2 env2,
+            evalExp e env = 0 →
+            Eval env s2 env2 →
+            Eval env (Stmt.If e s1 s2) env2
+| EWhileFalse : ∀ env e s1,
+            evalExp e env = 0 →
+            Eval env (Stmt.While e s1) env
+| EWhileTrue : ∀ env env1 env2 e s1 n,
+            evalExp e env = n + 1 →
+            Eval env s1 env1 →
+            Eval env1 (Stmt.While e s1) env2 →
+            Eval env (Stmt.While e s1) env2
+
+
+-- Hoare logic 
+
+def Hoare (P : Env → Prop)(s : Stmt)(Q : Env → Prop) :=
+  ∀ (env env' : Env), P env → Eval env s env' → Q env'
+
+macro "{*" P:term " *} " "(" s:term ")" " {* " Q:term " *}" : term =>
+  `(Hoare $P $s $Q)
+
+-- rules of Hoare logic 
+
+theorem Skip_rule (P : Env → Prop) 
+  : {* P *} (Stmt.Skip) {* P *}:= by 
+  intros env env' Hp Hev
+  cases Hev 
+  exact Hp 
+
+def assertion_sub (s : String) (e : IExp) (P : Env → Prop) : Env → Prop := 
+  λ env => P (s |-> (evalExp e env) ; env)
+
+macro P:term "[*" s:term "↦" e:term "*]" : term => 
+  `(assertion_sub $s $e $P)
+
+theorem Assign_rule (P : Env → Prop)
+  s e :   {* P [* s ↦ e *] *}
+            (Stmt.Assign s e) 
+          {* P *} := by 
+  intros env env' Hp H1
+  cases H1
+  rw [assertion_sub] at Hp
+  rename_i He 
+  rw [← He]
+  assumption
+
+
