Pcc116Code/LamRec.lean
@@ -1,0 +1,113 @@
+import Mathlib.Tactic.Basic 
+import Mathlib.Data.Nat.Defs
+
+-- infrastructure
+
+section DeBruijn
+  variable {A : Type}
+
+  inductive In : A → List A → Type where 
+  | Here : ∀ x xs, In x (x :: xs)
+  | There : ∀ x y ys, In x ys → In x (y :: ys)
+
+end DeBruijn
+
+-- syntax 
+
+inductive Ty : Type where 
+| Nat : Ty 
+| Arrow : Ty → Ty → Ty 
+| Rec : List Ty → Ty 
+
+abbrev Ctx := List Ty 
+
+mutual 
+
+  inductive Fields : Ctx → List Ty → Type where 
+  | Nil : ∀ ctx, Fields ctx []
+  | Cons : ∀ ctx t ts, Exp ctx t → 
+                       Fields ctx ts → 
+                       Fields ctx (t :: ts)
+
+  inductive Exp : Ctx → Ty → Type where 
+  | Num : ∀ ctx, ℕ → Exp ctx Ty.Nat 
+  | Var : ∀ ctx t, In t ctx → Exp ctx t 
+  | Abs : ∀ ctx t' t, Exp (t' :: ctx) t → 
+                      Exp ctx (Ty.Arrow t' t)
+  | App : ∀ ctx t t', Exp ctx (Ty.Arrow t' t) → 
+                      Exp ctx t' → 
+                      Exp ctx t 
+  | MkRec : ∀ ctx ts, Fields ctx ts → 
+                      Exp ctx (Ty.Rec ts)
+  | AccField : ∀ ctx t ts, Exp ctx (Ty.Rec ts) → 
+                           In t ts → 
+                           Exp ctx t 
+
+end
+
+-- semantics 
+
+mutual 
+  def semTy : Ty → Type 
+  | Ty.Nat => ℕ 
+  | Ty.Arrow t1 t2 => semTy t1 → semTy t2 
+  | Ty.Rec ts => semCtx ts 
+
+  def semCtx : List Ty → Type 
+  | [] => Unit 
+  | t :: ts => semTy t × semCtx ts 
+end 
+
+def lookupVar {ctx t} : In t ctx → semCtx ctx → semTy t
+| In.Here _ _, H => by 
+  simp [semCtx] at H 
+  rcases H with ⟨ H1, _H2 ⟩ 
+  exact H1 
+| In.There _ _ _ ix, H => by 
+  simp [semCtx] at H 
+  rcases H with ⟨ _H1, H2 ⟩ 
+  exact (lookupVar ix H2) 
+
+
+
+mutual
+  def evalExp {ctx t} : Exp ctx t → semCtx ctx → semTy t 
+  | Exp.Num _ n, _ => n
+  | Exp.Var _ _ v, env => lookupVar v env
+  | Exp.Abs _ _ _ e, env => by 
+    simp [semTy] 
+    intros v 
+    apply evalExp 
+    exact e 
+    simp [semCtx]
+    constructor <;> assumption
+  | Exp.App _ _ _ e1 e2, env => by 
+    have H1 : _ := by exact (evalExp e1 env)
+    have H2 : _ := by exact (evalExp e2 env)
+    simp only [semTy] at H1
+    simp only [semTy] at H2 
+    exact (H1 H2)
+  | Exp.MkRec _ _ fs, env => by 
+    simp [semTy] 
+    exact (evalFields fs env)
+  | Exp.AccField _ _ _ e v, env => by 
+    have H1 : _ := by exact (evalExp e env)
+    simp [semTy] at H1
+    exact (lookupVar v H1)
+  termination_by e env => sizeOf e
+  decreasing_by 
+    all_goals simp_wf
+    all_goals omega 
+
+  def evalFields {ctx ts} : Fields ctx ts → semCtx ctx → semCtx ts
+  | Fields.Nil _ , _ => Unit.unit
+  | Fields.Cons _ _ _ v fs, env => by 
+    simp [semCtx] 
+    constructor 
+    apply (evalExp v env) 
+    apply (evalFields fs env)
+  termination_by fs env => sizeOf fs
+  decreasing_by 
+    all_goals simp_wf 
+    all_goals omega 
+end 
