Pcc116Code/Regex.lean
@@ -1,0 +1,133 @@
+import Mathlib.Tactic.Basic
+import Mathlib.Data.Nat.Defs 
+import Aesop 
+
+inductive regex where 
+| empty : regex  
+| lambda : regex  
+| chr : Char → regex  
+| cat : regex → regex → regex 
+| choice : regex → regex → regex 
+| star : regex → regex 
+deriving Repr 
+
+inductive regex_match : List Char → regex → Prop where 
+| mlambda : regex_match [] regex.lambda  
+| mchr : ∀ c, regex_match [c] (regex.chr c)
+| mcat : ∀ e1 e2 s1 s2 s3, 
+  regex_match s1 e1 → 
+  regex_match s2 e2 → 
+  s3 = s1 ++ s2 → 
+  regex_match s3 (regex.cat e1 e2)
+| minl : ∀ e1 e2 s1, 
+  regex_match s1 e1 → 
+  regex_match s1 (regex.choice e1 e2)
+| minr : ∀ e1 e2 s2, 
+  regex_match s2 e2 → 
+  regex_match s2 (regex.choice e1 e2)
+| mnil : ∀ e1,
+  regex_match [] (regex.star e1)
+| mcons : ∀ e1 s1 ss1 s3, 
+  regex_match s1 e1 → 
+  regex_match ss1 (regex.star e1) → 
+  s3 = s1 ++ ss1 → 
+  regex_match s3 (regex.star e1)
+
+infix:60 " <<- " => regex_match 
+
+def nullable : regex → Bool 
+| regex.empty => false 
+| regex.lambda => true 
+| regex.chr _ => false 
+| regex.cat e1 e2 => nullable e1 && nullable e2 
+| regex.choice e1 e2 => 
+  nullable e1 || nullable e2 
+| regex.star _ => true 
+
+theorem nullable_sound 
+  : ∀ e, nullable e = true → [] <<- e := by 
+    intros e 
+    induction e with 
+    | empty => 
+      intros H 
+      simp [nullable] at H  
+    | lambda => 
+      intros _H
+      constructor 
+    | chr c =>
+      intros H 
+      simp [nullable] at H 
+    | cat e1 e2 IHe1 IHe2 =>
+      intros H 
+      simp [nullable] at H 
+      have Heq : @List.nil Char = [] ++ [] := by
+        simp
+      rw [Heq]
+      rcases H with ⟨ H1 , H2 ⟩ 
+      constructor
+      · 
+        apply IHe1 ; assumption 
+      · 
+        apply IHe2 ; assumption
+      · 
+        simp 
+    | choice e1 e2 IHe1 IHe2 => 
+      intros H 
+      simp [nullable] at H
+      rcases H with H1 | H2 
+      · 
+        apply regex_match.minl 
+        apply IHe1 ; assumption 
+      · 
+        apply regex_match.minr 
+        apply IHe2 ; assumption
+    | star e1 _IHe1 => 
+      intros _H
+      constructor
+
+theorem nullable_complete 
+  : ∀ e, [] <<- e → nullable e = true := by 
+    intros e 
+    induction e with 
+    | empty => 
+      intros H
+      cases H
+    | lambda =>
+      intros _H 
+      simp [nullable]
+    | chr c => 
+      intros H 
+      cases H 
+    | cat e1 e2 IHe1 IHe2 => 
+      intros H 
+      simp [nullable] 
+      rcases H 
+      rename_i H2 H1 Heq
+      simp [List.append_eq_nil] at H2
+      rcases H2 with ⟨ H2, H3 ⟩ 
+      constructor 
+      · 
+        apply IHe1 
+        simp [H2] at *
+        assumption
+      · 
+        apply IHe2 
+        simp [H3] at * 
+        assumption 
+    | choice e1 e2 IHe1 IHe2 =>
+      intros H 
+      simp [nullable]
+      rcases H 
+      · 
+        rename_i H1 
+        left 
+        apply IHe1 
+        assumption 
+      · 
+        rename_i H1 
+        right 
+        apply IHe2 
+        assumption 
+    | star e1 _IHe1 => 
+      intros _H 
+      simp [nullable]
